@prefix sec: <https://w3id.org/security/v1> .
@prefix cred: <https://w3.org/2018/credentials#> .
@prefix dc: <http://purl.org/dc/terms/> .
@prefix owl: <http://www.w3.org/2002/07/owl#> .
@prefix rdf: <http://www.w3.org/1999/02/22-rdf-syntax-ns#> .
@prefix rdfs: <http://www.w3.org/2000/01/rdf-schema#> .
@prefix xsd: <http://www.w3.org/2001/XMLSchema#> .

# Ontology definition
cred: a owl:Ontology ;
    dc:title """Security Vocabulary"""@en ;
    dc:description """vocabulary used to ensure the authenticity and integrity of Verifiable Credentials and similar types of constrained digital documents using cryptography, especially through the use of digital signatures and related mathematical proofs 
"""@en ;
    rdfs:seeAlso <https://www.w3.org/TR/vc-data-integrity/> ;
    dc:date "2022-11-15"^^xsd:date ;
.

# Class definitions
sec:Proof a rdfs:Class ;
    rdfs:label "Digital proof" ;
    rdfs:comment """This class represents a digital proof on serialized data. """@en ;
    rdfs:isDefinedBy cred: ;
.

sec:ProofGraph a rdfs:Class ;
    rdfs:label "An RDF Graph for a digital proof" ;
    rdfs:comment """Instances of this class are RDF Graphs, where each of these graphs must include exactly one Proof."""@en ;
    rdfs:isDefinedBy cred: ;
.

sec:VerificationMethod a rdfs:Class ;
    rdfs:label "Verification method" ;
    rdfs:comment """A Verification Method class can express different verification methods, such as cryptographic public keys, which can be used to authenticate or authorize interaction with the `controller` or associated parties. Verification methods might take many parameters."""@en ;
    rdfs:isDefinedBy cred: ;
.

sec:DataIntegrityProof a rdfs:Class ;
    rdfs:subClassOf sec:Proof ;
    rdfs:label "A Data Integrity Proof" ;
    rdfs:comment """This class represents a data integrity proof used to encode a variety of cryptographic suite proof encodings."""@en ;
    rdfs:isDefinedBy cred: ;
    rdfs:seeAlso <https://www.w3.org/TR/vc-data-integrity/#dataintegrityproof> ;
.

sec:Ed25519Signature2020 a rdfs:Class ;
    rdfs:subClassOf sec:Proof ;
    rdfs:label "ED2559 Signature Suite, 2020 version" ;
    rdfs:comment """T.B.D."""@en ;
    rdfs:isDefinedBy cred: ;
.

sec:Key a rdfs:Class, owl:DeprecatedClass ;
    owl:deprecated true ;
    rdfs:label "Cryptographic key" ;
    rdfs:comment """This class represents a cryptographic key that may be used for encryption, decryption, or digitally signing data."""@en ;
    rdfs:isDefinedBy cred: ;
.

sec:Signature a rdfs:Class, owl:DeprecatedClass ;
    owl:deprecated true ;
    rdfs:subClassOf sec:Proof ;
    rdfs:label "Digital signature" ;
    rdfs:comment """This class represents a digital signature on serialized data. It is an abstract class and should not be used other than for Semantic Web reasoning purposes, such as by a reasoning agent. This class MUST NOT be used directly, but only through its subclasses."""@en ;
    rdfs:isDefinedBy cred: ;
.

sec:SignatureGraph a rdfs:Class, owl:DeprecatedClass ;
    owl:deprecated true ;
    rdfs:subClassOf sec:ProofGraph ;
    rdfs:label "An RDF Graph for a digital signature" ;
    rdfs:comment """Instances of this class are RDF Graphs, where each of these graphs must include exactly one Signature."""@en ;
    rdfs:isDefinedBy cred: ;
.

sec:EcdsaSecp256k1Signature2019 a rdfs:Class, owl:DeprecatedClass ;
    owl:deprecated true ;
    rdfs:subClassOf sec:Signature ;
    rdfs:label "TBD." ;
    rdfs:comment """This class represents a data integrity signature suite."""@en ;
    rdfs:isDefinedBy cred: ;
    rdfs:seeAlso <https://w3c-ccg.github.io/ld-cryptosuite-registry/#ecdsa-secp256k1> ;
.

sec:EcdsaSecp256k1Signature2020 a rdfs:Class, owl:DeprecatedClass ;
    owl:deprecated true ;
    rdfs:subClassOf sec:Signature ;
    rdfs:label "TBD." ;
    rdfs:comment """This class represents a data integrity signature suite."""@en ;
    rdfs:isDefinedBy cred: ;
    rdfs:seeAlso <https://w3c-ccg.github.io/ld-cryptosuite-registry/#ecdsa-secp256k1> ;
.

sec:EcdsaSecp256k1RecoverySignature2020 a rdfs:Class, owl:DeprecatedClass ;
    owl:deprecated true ;
    rdfs:subClassOf sec:Signature ;
    rdfs:label "TBD." ;
    rdfs:comment """This class represents a data integrity signature."""@en ;
    rdfs:isDefinedBy cred: ;
    rdfs:seeAlso <https://w3c-ccg.github.io/ld-cryptosuite-registry/#ecdsasecp256k1recoverysignature2020> ;
.

sec:EcdsaSecp256k1VerificationKey2019 a rdfs:Class, owl:DeprecatedClass ;
    owl:deprecated true ;
    rdfs:subClassOf sec:Key ;
    rdfs:label "TBD." ;
    rdfs:comment """This class represents a data integrity verification method."""@en ;
    rdfs:isDefinedBy cred: ;
    rdfs:seeAlso <https://w3c-ccg.github.io/ld-cryptosuite-registry/#ecdsa-secp256k1> ;
.

sec:EcdsaSecp256k1RecoveryMethod2020 a rdfs:Class, owl:DeprecatedClass ;
    owl:deprecated true ;
    rdfs:subClassOf sec:Key ;
    rdfs:label "TBD." ;
    rdfs:comment """This class represents a data integrity verification method."""@en ;
    rdfs:isDefinedBy cred: ;
    rdfs:seeAlso <https://w3c-ccg.github.io/ld-cryptosuite-registry/#ecdsasecp256k1recoverymethod2020> ;
.

sec:RsaSignature2018 a rdfs:Class, owl:DeprecatedClass ;
    owl:deprecated true ;
    rdfs:subClassOf sec:Signature ;
    rdfs:label "Signature Suite for RSA (was deprecated in the CCG document)" ;
    rdfs:comment """This class represents a data integrity signature suite."""@en ;
    rdfs:isDefinedBy cred: ;
    rdfs:seeAlso <https://w3c-ccg.github.io/ld-cryptosuite-registry/#rsa> ;
.

sec:RsaVerificationKey2018 a rdfs:Class, owl:DeprecatedClass ;
    owl:deprecated true ;
    rdfs:subClassOf sec:Key ;
    rdfs:label "Verification Key for RSA (was deprecated in the CCG document)" ;
    rdfs:comment """This class represents a data integrity verification method."""@en ;
    rdfs:isDefinedBy cred: ;
    rdfs:seeAlso <https://w3c-ccg.github.io/ld-cryptosuite-registry/#rsa> ;
.

sec:SchnorrSecp256k1Signature2019 a rdfs:Class, owl:DeprecatedClass ;
    owl:deprecated true ;
    rdfs:subClassOf sec:Signature ;
    rdfs:label "TBD." ;
    rdfs:comment """This class represents a data integrity signature suite."""@en ;
    rdfs:isDefinedBy cred: ;
.

sec:SchnorrSecp256k1VerificationKey2019 a rdfs:Class, owl:DeprecatedClass ;
    owl:deprecated true ;
    rdfs:subClassOf sec:Key ;
    rdfs:label "TBD." ;
    rdfs:comment """This class represents a data integrity verification method."""@en ;
    rdfs:isDefinedBy cred: ;
.

sec:ServiceEndpointProxyService a rdfs:Class, owl:DeprecatedClass ;
    owl:deprecated true ;
    rdfs:label "TBD." ;
    rdfs:comment """T.B.D."""@en ;
    rdfs:isDefinedBy cred: ;
.

sec:Digest a rdfs:Class, owl:DeprecatedClass ;
    owl:deprecated true ;
    rdfs:label "Message digest" ;
    rdfs:comment """This class represents a message digest that may be used for data integrity verification. The digest algorithm used will determine the cryptographic properties of the digest."""@en ;
    rdfs:isDefinedBy cred: ;
.

sec:EncryptedMessage a rdfs:Class, owl:DeprecatedClass ;
    owl:deprecated true ;
    rdfs:label "Encrypted message" ;
    rdfs:comment """A class of messages that are obfuscated in some cryptographic manner. These messages are incredibly difficult to decrypt without the proper decryption key."""@en ;
    rdfs:isDefinedBy cred: ;
.

sec:GraphSignature2012 a rdfs:Class, owl:DeprecatedClass ;
    owl:deprecated true ;
    rdfs:subClassOf sec:Signature ;
    rdfs:label "RDF graph signature" ;
    rdfs:comment """A graph signature is used for digital signatures on RDF graphs. The default canonicalization mechanism is specified in the RDF Graph normalization specification, which effectively deterministically names all unnamed nodes. The default signature mechanism uses a SHA-256 digest and RSA to perform the digital signature."""@en ;
    rdfs:isDefinedBy cred: ;
.

sec:LinkedDataSignature2015 a rdfs:Class, owl:DeprecatedClass ;
    owl:deprecated true ;
    rdfs:subClassOf sec:Signature ;
    rdfs:label "Linked data signature, 2015 version (was deprecated in the CCG document)" ;
    rdfs:comment """A Linked Data signature is used for digital signatures on RDF Datasets. The default canonicalization mechanism is specified in the RDF Dataset Normalization specification, which effectively deterministically names all unnamed nodes. The default signature mechanism uses a SHA-256 digest and RSA to perform the digital signature."""@en ;
    rdfs:isDefinedBy cred: ;
.

sec:LinkedDataSignature2016 a rdfs:Class, owl:DeprecatedClass ;
    owl:deprecated true ;
    rdfs:subClassOf sec:Signature ;
    rdfs:label "Linked data signature, 2016 version (was deprecated in the CCG document)" ;
    rdfs:comment """A Linked Data signature is used for digital signatures on RDF Datasets. The default canonicalization mechanism is specified in the RDF Dataset Normalization specification, which effectively deterministically names all unnamed nodes. The default signature mechanism uses a SHA-256 digest and RSA to perform the digital signature."""@en ;
    rdfs:isDefinedBy cred: ;
.

sec:MerkleProof2019 a rdfs:Class, owl:DeprecatedClass ;
    owl:deprecated true ;
    rdfs:subClassOf sec:Signature ;
    rdfs:label "Merkle Proof" ;
    rdfs:comment """Linked Data signature is used for digital signatures on RDF Datasets. The default canonicalization mechanism is specified in the RDF Dataset Normalization specification, which effectively deterministically names all unnamed nodes. The default signature mechanism uses a SHA-256 digest and ECDSA to perform the digital signature."""@en ;
    rdfs:isDefinedBy cred: ;
    rdfs:seeAlso <https://w3c-ccg.github.io/lds-merkle-proof-2019/> ;
.

sec:X25519KeyAgreementKey2019 a rdfs:Class, owl:DeprecatedClass ;
    owl:deprecated true ;
    rdfs:subClassOf sec:Key ;
    rdfs:label "X25519 Key Agreement Key 2019" ;
    rdfs:comment """This class represents a verification key."""@en ;
    rdfs:isDefinedBy cred: ;
.

sec:Ed25519VerificationKey2018 a rdfs:Class, owl:DeprecatedClass ;
    owl:deprecated true ;
    rdfs:subClassOf sec:Key ;
    rdfs:label "ED2559 Verification Key, 2018 version" ;
    rdfs:comment """This class represents a data integrity verification method."""@en ;
    rdfs:isDefinedBy cred: ;
    rdfs:seeAlso <https://w3c-ccg.github.io/ld-cryptosuite-registry/#ed25519> ;
.

sec:Ed25519VerificationKey2020 a rdfs:Class, owl:DeprecatedClass ;
    owl:deprecated true ;
    rdfs:subClassOf sec:Key ;
    rdfs:label "ED2559 Verification Key, 2020 version" ;
    rdfs:comment """A linked data proof suite verification method type used with `Ed25519Signature2020`."""@en ;
    rdfs:isDefinedBy cred: ;
.

sec:JsonWebKey2020 a rdfs:Class, owl:DeprecatedClass ;
    owl:deprecated true ;
    rdfs:subClassOf sec:Key ;
    rdfs:label "JSON Web Key, 2020 version" ;
    rdfs:comment """A linked data proof suite verification method type used with `JsonWebSignature2020`"""@en ;
    rdfs:isDefinedBy cred: ;
.

sec:JsonWebSignature2020 a rdfs:Class, owl:DeprecatedClass ;
    owl:deprecated true ;
    rdfs:subClassOf sec:Signature ;
    rdfs:label "JSON Web Signature, 2020 version" ;
    rdfs:comment """A Linked Data signature is used for digital signatures on RDF Datasets. The default canonicalization mechanism is specified in the RDF Dataset Normalization specification, which deterministically names all unnamed nodes. The default signature mechanism uses a SHA-256 digest and JWS to perform the digital signature."""@en ;
    rdfs:isDefinedBy cred: ;
.

sec:BbsBlsSignature2020 a rdfs:Class, owl:DeprecatedClass ;
    owl:deprecated true ;
    rdfs:subClassOf sec:Signature ;
    rdfs:label "BBS Signature, 2020 version" ;
    rdfs:comment """A Linked Data signature is used for digital signatures on RDF Datasets. The default canonicalization mechanism is specified in the RDF Dataset Normalization specification, which deterministically names all unnamed nodes. Importantly, a `BbsBlsSignature` digests each of the statements produced by the normalization process individually to enable selective disclosure. The signature mechanism uses Blake2B as the digest for each statement and produces a single output digital signature."""@en ;
    rdfs:isDefinedBy cred: ;
.

sec:BbsBlsSignatureProof2020 a rdfs:Class, owl:DeprecatedClass ;
    owl:deprecated true ;
    rdfs:subClassOf sec:Signature ;
    rdfs:label "BBS Signature Proof, 2020 version" ;
    rdfs:comment """A Linked Data signature is used for digital signatures on RDF Datasets. The default canonicalization mechanism is specified in the RDF Dataset Normalization specification, which deterministically names all unnamed nodes. Importantly, a `BbsBlsSignatureProof2020` is in fact a proof of knowledge of an unrevealed BbsBlsSignature2020 enabling the ability to selectively reveal information from the set that was originally signed. Each of the statements produced by the normalizing process for a JSON-LD document featuring a `BbsBlsSignatureProof2020` represent statements that were originally signed in producing the `BbsBlsSignature2020` and represent the denomination under which information can be selectively disclosed. The signature mechanism uses Blake2B as the digest for each statement and produces a single output digital signature."""@en ;
    rdfs:isDefinedBy cred: ;
.

sec:Bls12381G1Key2020 a rdfs:Class, owl:DeprecatedClass ;
    owl:deprecated true ;
    rdfs:subClassOf sec:Key ;
    rdfs:label "BLS 12381 G1 Signature Key, 2020 version" ;
    rdfs:comment """This class represents a data integrity signature key."""@en ;
    rdfs:isDefinedBy cred: ;
    rdfs:seeAlso <https://w3c-ccg.github.io/ld-cryptosuite-registry/#ed25519> ;
.

sec:Bls12381G2Key2020 a rdfs:Class, owl:DeprecatedClass ;
    owl:deprecated true ;
    rdfs:subClassOf sec:Key ;
    rdfs:label "BLS 12381 G2 Signature Key, 2020 version" ;
    rdfs:comment """This class represents a data integrity signature key."""@en ;
    rdfs:isDefinedBy cred: ;
    rdfs:seeAlso <https://w3c-ccg.github.io/ld-cryptosuite-registry/#ed25519> ;
.



# Property definitions
sec:proofPurpose a rdfs:Property, owl:DatatypeProperty ;
    rdfs:domain sec:Proof ;
    rdfs:range xsd:string ;
    rdfs:label "Proof purpose" ;
    rdfs:comment """The` proofPurpose` property is used to associate a purpose, such as `assertionMethod` or `authentication` with a proof. The proof purpose acts as a safeguard to prevent the proof from being misused by being applied to a purpose other than the one that was intended."""@en ;
    rdfs:isDefinedBy cred: ;
.

sec:verificationMethod a rdfs:Property ;
    rdfs:range sec:VerificationMethod ;
    rdfs:label "Verification method" ;
    rdfs:comment """A `verificationMethod` property is used to specify a URL that contains information used for proof verification."""@en ;
    rdfs:isDefinedBy cred: ;
    rdfs:seeAlso <https://www.w3.org/TR/did-core/#verification-methods> ;
.

sec:created a rdfs:Property, owl:DatatypeProperty ;
    rdfs:domain sec:Proof ;
    rdfs:range xsd:dateTime ;
    rdfs:label "Creation date of the proof" ;
    rdfs:comment """The date and time the proof was created. This information MUST be added to a proof."""@en ;
    rdfs:isDefinedBy cred: ;
.

sec:domain a rdfs:Property, owl:DatatypeProperty ;
    rdfs:domain sec:Proof ;
    rdfs:range xsd:string ;
    rdfs:label "Domain of a proof" ;
    rdfs:comment """The `domain` property is used to associate a domain with a proof, for use with a `proofPurpose` such as `authentication` and indicating its intended usage."""@en ;
    rdfs:isDefinedBy cred: ;
.

sec:challenge a rdfs:Property, owl:DatatypeProperty ;
    rdfs:domain sec:Proof ;
    rdfs:range xsd:string ;
    rdfs:label "Challenge with a proof" ;
    rdfs:comment """The challenge property is used to associate a challenge with a proof, for use with a `proofPurpose` such as `authentication`. This string value SHOULD be included in a proof if a `domain` is specified."""@en ;
    rdfs:isDefinedBy cred: ;
.

sec:proofPurpose a rdfs:Property, owl:DatatypeProperty ;
    rdfs:domain sec:Proof ;
    rdfs:range xsd:string ;
    rdfs:label "Proof purpose" ;
    rdfs:comment """The` proofPurpose` property is used to associate a purpose, such as `assertionMethod` or `authentication` with a proof. The proof purpose acts as a safeguard to prevent the proof from being misused by being applied to a purpose other than the one that was intended."""@en ;
    rdfs:isDefinedBy cred: ;
.

sec:proofValue a rdfs:Property, owl:DatatypeProperty ;
    rdfs:domain sec:Proof ;
    rdfs:range xsd:string ;
    rdfs:label "Proof value" ;
    rdfs:comment """A string value that contains the data necessary to verify the digital proof using the `verificationMethod` specified"""@en ;
    rdfs:isDefinedBy cred: ;
.

sec:proof a rdfs:Property ;
    rdfs:range sec:ProofGraph ;
    rdfs:label "Proof sets" ;
    rdfs:comment """The value of the `proof` property MUST identify `ProofGraph` instances (informally, it indirectly identifies `Proof` instances each contained in a separate graph). The property is used to associate a proof with a graph of information. The proof property is typically not included in the canonicalized graphs that are then digested, and digitally signed. The order of the proofs is not relevant."""@en ;
    rdfs:isDefinedBy cred: ;
.

sec:proofChain a rdfs:Property ;
    rdfs:range rdf:List ;
    rdfs:label "Proof chain" ;
    rdfs:comment """The value of the `proofChain` property MUST identify a sequence of `ProofGraph` instances (informally, it indirectly identifies a series of `Proof` instances, each contained in a separate graph). The property is used to provide a sequence of multiple proofs where the order of when the proofs occurred matters. The proof chain property is typically not included in the canonicalized graphs that are then separately digested, and digitally signed."""@en ;
    rdfs:isDefinedBy cred: ;
.

sec:controller a rdfs:Property, owl:ObjectProperty ;
    rdfs:domain sec:VerificationMethod ;
    rdfs:range  ;
    rdfs:label "Controller" ;
    rdfs:comment """A controller is an entity that claims control over a particular resource. Note that control is best validated as a two-way relationship where the controller claims control over a particular resource, and the resource clearly identifies its controller."""@en ;
    rdfs:isDefinedBy cred: ;
.

sec:publicKeyJwk a rdfs:Property, owl:DatatypeProperty ;
    rdfs:domain sec:VerificationMethod ;
    rdfs:range xsd:string ;
    rdfs:label "Public key JWK" ;
    rdfs:comment """See the JOSE suite."""@en ;
    rdfs:isDefinedBy cred: ;
    rdfs:seeAlso <https://www.iana.org/assignments/jose/jose.xhtml>, <https://tools.ietf.org/html/rfc7517> ;
.

sec:publicKeyMultibase a rdfs:Property, owl:DatatypeProperty ;
    rdfs:domain sec:VerificationMethod ;
    rdfs:range xsd:string ;
    rdfs:label "Public key multibase" ;
    rdfs:comment """The public key multibase property is used to specify the multibase-encoded version of a public key. The contents of the property are defined by specifications such as ED25519-2020 and listed in the Linked Data Cryptosuite Registry. Most public key type definitions are expected to:
• Specify only a single encoding base per public key type as it reduces implementation burden and increases the chances of reaching broad interoperability.
• Specify a multicodec header on the encoded public key to aid encoding and decoding applications in confirming that they are serializing and deserializing an expected public key type.
• Use compressed binary formats to ensure efficient key sizes."""@en ;
    rdfs:isDefinedBy cred: ;
    rdfs:seeAlso <https://datatracker.ietf.org/doc/html/draft-multiformats-multibase-03>, <https://w3c-ccg.github.io/ld-cryptosuite-registry/>, <https://github.com/multiformats/multicodec/blob/master/table.csv>, <https://w3c-ccg.github.io/lds-ed25519-2020/> ;
.

sec:authentication a rdfs:Property ;
    rdfs:range VerificationMethod ;
    rdfs:label "Authentication method" ;
    rdfs:comment """An `authentication` property is used to specify a URL that contains information about a `verificationMethod` used for authentication."""@en ;
    rdfs:isDefinedBy cred: ;
.

sec:assertionMethod a rdfs:Property ;
    rdfs:range VerificationMethod ;
    rdfs:label "Assertion method" ;
    rdfs:comment """An `assertionMethod` property is used to specify a URL that contains information about a `verificationMethod` used for assertions."""@en ;
    rdfs:isDefinedBy cred: ;
.

sec:capabilityDelegation a rdfs:Property ;
    rdfs:range VerificationMethod ;
    rdfs:label "Capability Delegation Method" ;
    rdfs:comment """A `capabilityDelegation` property is used to express that one or more `verificationMethods` are authorized to verify cryptographic proofs that were created for the purpose of delegating capabilities.
A `verificationMethod` may be referenced by its identifier (a URL) or expressed in full.
The aforementioned proofs are created to prove that some entity is delegating the authority to take some action to another entity. A verifier of the proof should expect the proof to express a `proofPurpose` of `capabilityDelegation` and reference a `verificationMethod` to verify it. The dereferenced `verificationMethod` MUST have a controller property that has a property of `capabilityDelegation` that references the `verificationMethod`. This indicates that the controller has authorized it for the expressed `proofPurpose`."""@en ;
    rdfs:isDefinedBy cred: ;
.

sec:capabilityInvocation a rdfs:Property ;
    rdfs:range VerificationMethod ;
    rdfs:label "Capability Invocation Method" ;
    rdfs:comment """A `capabilityInvocation` property is used to express that one or more `verificationMethods` are authorized to verify cryptographic proofs that were created for the purpose of invoking capabilities.
A `verificationMethod` MAY be referenced by its identifier (a URL) or expressed in full.
The aforementioned proofs are created to prove that some entity is attempting to exercise some authority they possess to take an action. A verifier of the proof should expect the proof to express a `proofPurpose` of `capabilityInvocation` and reference a `verificationMethod` to verify it. The dereferenced `verificationMethod` MUST have a controller property that, when dereferenced, has a property of `capabilityInvocation` that references the `verificationMethod.` This indicates that the controller has authorized it for the expressed `proofPurpose`."""@en ;
    rdfs:isDefinedBy cred: ;
.

sec:keyAgreement a rdfs:Property ;
    rdfs:range VerificationMethod ;
    rdfs:label "Key agreement protocols" ;
    rdfs:comment """Indicates that a proof is used for for key agreement protocols, such as Elliptic Curve Diffie Hellman key agreement used by popular encryption libraries."""@en ;
    rdfs:isDefinedBy cred: ;
.

sec:cryptosuite a rdfs:Property, owl:DatatypeProperty ;
    rdfs:domain sec:DataIntegrityProof ;
    rdfs:range xsd:string ;
    rdfs:label "Cryptographic suite" ;
    rdfs:comment """A text-based identifier for a specific cryptographic suite."""@en ;
    rdfs:isDefinedBy cred: ;
    rdfs:seeAlso <https://www.w3.org/TR/vc-data-integrity/#dataintegrityproof> ;
.

sec:publicKeyMultibase a rdfs:Property, owl:DatatypeProperty ;
    rdfs:domain sec:VerificationMethod ;
    rdfs:range xsd:string ;
    rdfs:label "Public key multibase" ;
    rdfs:comment """The public key multibase property is used to specify the multibase-encoded version of a public key. The contents of the property are defined by specifications such as ED25519-2020 and listed in the Linked Data Cryptosuite Registry. Most public key type definitions are expected to:
• Specify only a single encoding base per public key type as it reduces implementation burden and increases the chances of reaching broad interoperability.
• Specify a multicodec header on the encoded public key to aid encoding and decoding applications in confirming that they are serializing and deserializing an expected public key type.
• Use compressed binary formats to ensure efficient key sizes."""@en ;
    rdfs:isDefinedBy cred: ;
    rdfs:seeAlso <https://datatracker.ietf.org/doc/html/draft-multiformats-multibase-03>, <https://w3c-ccg.github.io/ld-cryptosuite-registry/>, <https://github.com/multiformats/multicodec/blob/master/table.csv>, <https://w3c-ccg.github.io/lds-ed25519-2020/> ;
.

sec:publicKeyJwk a rdfs:Property, owl:DatatypeProperty ;
    rdfs:domain sec:VerificationMethod ;
    rdfs:range xsd:string ;
    rdfs:label "Public key JWK" ;
    rdfs:comment """See the JOSE suite."""@en ;
    rdfs:isDefinedBy cred: ;
    rdfs:seeAlso <https://www.iana.org/assignments/jose/jose.xhtml>, <https://tools.ietf.org/html/rfc7517> ;
.

sec:cipherAlgorithm a rdf:Property, owl:DeprecatedProperty, owl:DatatypeProperty ;
    owl:deprecated true ;
    rdfs:domain sec:EncryptedMessage ;
    rdfs:range xsd:string ;
    rdfs:label "Cipher algorithm" ;
    rdfs:comment """The cipher algorithm describes the mechanism used to encrypt a message. It is typically a string expressing the cipher suite, the strength of the cipher, and a block cipher mode."""@en ;
    rdfs:isDefinedBy cred: ;
.

sec:cipherData a rdf:Property, owl:DeprecatedProperty, owl:DatatypeProperty ;
    owl:deprecated true ;
    rdfs:domain sec:EncryptedMessage ;
    rdfs:range xsd:string ;
    rdfs:label "Cipher data" ;
    rdfs:comment """Cipher data is an opaque blob of information that is used to specify an encrypted message."""@en ;
    rdfs:isDefinedBy cred: ;
.

sec:cipherKey a rdf:Property, owl:DeprecatedProperty, owl:DatatypeProperty ;
    owl:deprecated true ;
    rdfs:domain sec:EncryptedMessage ;
    rdfs:range xsd:string ;
    rdfs:label "Cipher key" ;
    rdfs:comment """A cipher key is a symmetric key that is used to encrypt or decrypt a piece of information. The key itself may be expressed in clear text or encrypted."""@en ;
    rdfs:isDefinedBy cred: ;
.

sec:digestAlgorithm a rdf:Property, owl:DeprecatedProperty, owl:DatatypeProperty ;
    owl:deprecated true ;
    rdfs:range xsd:string ;
    rdfs:label "Digest algorithm" ;
    rdfs:comment """The digest algorithm is used to specify the cryptographic function to use when generating the data to be digitally signed. Typically, data that is to be signed goes through three steps: 1) canonicalization, 2) digest, and 3) signature. This property is used to specify the algorithm that should be used for step 2. A signature class typically specifies a default digest method, so this property is typically used to specify information for a signature algorithm."""@en ;
    rdfs:isDefinedBy cred: ;
.

sec:digestValue a rdf:Property, owl:DeprecatedProperty, owl:DatatypeProperty ;
    owl:deprecated true ;
    rdfs:range xsd:string ;
    rdfs:label "Digest value" ;
    rdfs:comment """The digest value is used to express the output of the digest algorithm expressed in Base-16 (hexadecimal) format."""@en ;
    rdfs:isDefinedBy cred: ;
.

sec:blockchainAccountId a rdf:Property, owl:DeprecatedProperty, owl:DatatypeProperty ;
    owl:deprecated true ;
    rdfs:range xsd:string ;
    rdfs:label "Blockchain account ID" ;
    rdfs:comment """A `blockchainAccountId` property is used to specify a blockchain account identifier, as per the CAIP-10Account ID Specification."""@en ;
    rdfs:isDefinedBy cred: ;
.

sec:ethereumAddress a rdf:Property, owl:DeprecatedProperty, owl:DatatypeProperty ;
    owl:deprecated true ;
    rdfs:range xsd:string ;
    rdfs:label "Ethereum address" ;
    rdfs:comment """An `ethereumAddress` property is used to specify the Ethereum address. As per the Ethereum Yellow Paper “Ethereum: a secure decentralised generalised transaction ledger” in consists of a prefix "0x", a common identifier for hexadecimal, concatenated with the rightmost 20 bytes of the Keccak-256 hash (big endian) of the ECDSA public key (the curve used is the so-called secp256k1). In hexadecimal, 2 digits represent a byte, meaning addresses contain 40 hexadecimal digits. The Ethereum address should also contain a checksum as per EIP-55."""@en ;
    rdfs:isDefinedBy cred: ;
    rdfs:seeAlso <https://eips.ethereum.org/EIPS/eip-55>, <https://ethereum.github.io/yellowpaper/paper.pdf> ;
.

sec:expires a rdf:Property, owl:DeprecatedProperty, owl:DatatypeProperty ;
    owl:deprecated true ;
    rdfs:range xsd:dateTime ;
    rdfs:label "Expiration time" ;
    rdfs:comment """The expiration time is typically associated with a `Key` and specifies when the validity of the key will expire."""@en ;
    rdfs:isDefinedBy cred: ;
.

sec:initializationVector a rdf:Property, owl:DeprecatedProperty, owl:DatatypeProperty ;
    owl:deprecated true ;
    rdfs:domain sec:EncryptedMessage ;
    rdfs:range xsd:string ;
    rdfs:label "Initialization vector" ;
    rdfs:comment """The initialization vector (IV) is a byte stream that is typically used to initialize certain block cipher encryption schemes. For a receiving application to be able to decrypt a message, it must know the decryption key and the initialization vector. The value is typically base-64 encoded."""@en ;
    rdfs:isDefinedBy cred: ;
.

sec:nonce a rdf:Property, owl:DeprecatedProperty, owl:DatatypeProperty ;
    owl:deprecated true ;
    rdfs:domain sec:Signature ;
    rdfs:range xsd:string ;
    rdfs:label "Nonce" ;
    rdfs:comment """This property is used in conjunction with the input to the signature hashing function in order to protect against replay attacks. Typically, receivers need to track all nonce values used within a certain time period in order to ensure that an attacker cannot merely re-send a compromised packet in order to execute a privileged request."""@en ;
    rdfs:isDefinedBy cred: ;
.

sec:canonicalizationAlgorithm a rdf:Property, owl:DeprecatedProperty ;
    owl:deprecated true ;
    rdfs:domain sec:Signature ;
    rdfs:label "Canonicalization algorithm" ;
    rdfs:comment """The canonicalization algorithm is used to transform the input data into a form that can be passed to a cryptographic digest method. The digest is then digitally signed using a digital signature algorithm. Canonicalization ensures that a piece of software that is generating a digital signature is able to do so on the same set of information in a deterministic manner."""@en ;
    rdfs:isDefinedBy cred: ;
.

sec:controller a rdf:Property, owl:DeprecatedProperty, owl:ObjectProperty ;
    owl:deprecated true ;
    rdfs:range  ;
    rdfs:label "Controller" ;
    rdfs:comment """A controller is an entity that claims control over a particular resource. Note that control is best validated as a two-way relationship where the controller claims control over a particular resource, and the resource clearly identifies its controller."""@en ;
    rdfs:isDefinedBy cred: ;
.

sec:owner a rdf:Property, owl:DeprecatedProperty, owl:ObjectProperty ;
    owl:deprecated true ;
    rdfs:range  ;
    rdfs:label "Owner (was deprecated in the CCG document)" ;
    rdfs:comment """An owner is an entity that claims control over a particular resource. Note that ownership is best validated as a two-way relationship where the owner claims ownership over a particular resource, and the resource clearly identifies its owner."""@en ;
    rdfs:isDefinedBy cred: ;
.

sec:password a rdf:Property, owl:DeprecatedProperty, owl:DatatypeProperty ;
    owl:deprecated true ;
    rdfs:range xsd:string ;
    rdfs:label "Password" ;
    rdfs:comment """A secret that is used to generate a key that can be used to encrypt or decrypt message. It is typically a string value."""@en ;
    rdfs:isDefinedBy cred: ;
.

sec:privateKeyPem a rdf:Property, owl:DeprecatedProperty, owl:DatatypeProperty ;
    owl:deprecated true ;
    rdfs:domain sec:Key ;
    rdfs:range xsd:string ;
    rdfs:label "PEM encoded private key" ;
    rdfs:comment """A private key PEM property is used to specify the PEM-encoded version of the private key. This encoding is compatible with almost every Secure Sockets Layer library implementation and typically plugs directly into functions intializing private keys."""@en ;
    rdfs:isDefinedBy cred: ;
    rdfs:seeAlso <http://en.wikipedia.org/wiki/Privacy_Enhanced_Mail> ;
.

sec:publicKey a rdf:Property, owl:DeprecatedProperty, owl:ObjectProperty ;
    owl:deprecated true ;
    rdfs:domain sec:Key ;
    rdfs:range  ;
    rdfs:label "Public Key" ;
    rdfs:comment """A public key property is used to specify a URL that contains information about a public key."""@en ;
    rdfs:isDefinedBy cred: ;
.

sec:publicKeyBase58 a rdf:Property, owl:DeprecatedProperty, owl:DatatypeProperty ;
    owl:deprecated true ;
    rdfs:domain sec:Key ;
    rdfs:range xsd:string ;
    rdfs:label "Base58-encoded Public Key" ;
    rdfs:comment """A public key Base58 property is used to specify the base58-encoded version of the public key."""@en ;
    rdfs:isDefinedBy cred: ;
.

sec:publicKeyPem a rdf:Property, owl:DeprecatedProperty, owl:DatatypeProperty ;
    owl:deprecated true ;
    rdfs:domain sec:Key ;
    rdfs:range xsd:string ;
    rdfs:label "Public key PEM" ;
    rdfs:comment """A public key PEM property is used to specify the PEM-encoded version of the public key. This encoding is compatible with almost every Secure Sockets Layer library implementation and typically plugs directly into functions initializing public keys."""@en ;
    rdfs:isDefinedBy cred: ;
.

sec:publicKeyHex a rdf:Property, owl:DeprecatedProperty, owl:DatatypeProperty ;
    owl:deprecated true ;
    rdfs:domain sec:Key ;
    rdfs:range xsd:string ;
    rdfs:label "Hex-encoded version of public Key" ;
    rdfs:comment """A `publicKeyHex` property is used to specify the hex-encoded version of the public key, based on section 8 of rfc4648. Hex encoding is also known as Base16 encoding."""@en ;
    rdfs:isDefinedBy cred: ;
    rdfs:seeAlso <https://tools.ietf.org/html/rfc4648#section-8> ;
.

sec:publicKeyService a rdf:Property, owl:DeprecatedProperty, owl:ObjectProperty ;
    owl:deprecated true ;
    rdfs:range  ;
    rdfs:label "Public key service" ;
    rdfs:comment """The publicKeyService property is used to express the REST URL that provides public key management services."""@en ;
    rdfs:isDefinedBy cred: ;
.

sec:revoked a rdf:Property, owl:DeprecatedProperty, owl:DatatypeProperty ;
    owl:deprecated true ;
    rdfs:range xsd:dateTime ;
    rdfs:label "Revocation time" ;
    rdfs:comment """The revocation time is typically associated with a `Key` that has been marked as invalid as of the date and time associated with the property. Key revocations are often used when a key is compromised, such as the theft of the private key, or during the course of best-practice key rotation schedules."""@en ;
    rdfs:isDefinedBy cred: ;
.

sec:jws a rdf:Property, owl:DeprecatedProperty ;
    owl:deprecated true ;
    rdfs:range sec:Signature ;
    rdfs:label "Json Web Signature" ;
    rdfs:comment """The jws property is used to associate a detached Json Web Signature with a proof."""@en ;
    rdfs:isDefinedBy cred: ;
    rdfs:seeAlso <https://tools.ietf.org/html/rfc7797> ;
.

sec:challenge a rdf:Property, owl:DeprecatedProperty, owl:DatatypeProperty ;
    owl:deprecated true ;
    rdfs:domain sec:Proof ;
    rdfs:range xsd:string ;
    rdfs:label "Challenge with a proof" ;
    rdfs:comment """The challenge property is used to associate a challenge with a proof, for use with a `proofPurpose` such as `authentication`. This string value SHOULD be included in a proof if a `domain` is specified."""@en ;
    rdfs:isDefinedBy cred: ;
.

sec:expirationDate a rdf:Property, owl:DeprecatedProperty, owl:DatatypeProperty ;
    owl:deprecated true ;
    rdfs:domain sec:Proof ;
    rdfs:range xsd:dateTime ;
    rdfs:label "Expiration date for proof" ;
    rdfs:comment """The `expirationDate` property is used to associate an expiration date with a proof."""@en ;
    rdfs:isDefinedBy cred: ;
.

sec:signature a rdf:Property, owl:DeprecatedProperty ;
    owl:deprecated true ;
    rdfs:range sec:Signature ;
    rdfs:label "Signature  (was deprecated in the CCG document)" ;
    rdfs:comment """The property is used to associate a proof with a graph of information. The proof property is typically not included in the canonicalized graph that is then digested, and digitally signed."""@en ;
    rdfs:isDefinedBy cred: ;
.

sec:signatureValue a rdf:Property, owl:DeprecatedProperty, owl:DatatypeProperty ;
    owl:deprecated true ;
    rdfs:domain sec:Signature ;
    rdfs:range xsd:string ;
    rdfs:label "Signature value  (was deprecated in the CCG document)" ;
    rdfs:comment """The signature value is used to express the output of the signature algorithm expressed in base-64 format."""@en ;
    rdfs:isDefinedBy cred: ;
.

sec:signatureAlgorithm a rdf:Property, owl:DeprecatedProperty, owl:ObjectProperty ;
    owl:deprecated true ;
    rdfs:domain sec:Signature ;
    rdfs:range  ;
    rdfs:label "Signature algorithm  (was deprecated in the CCG document)" ;
    rdfs:comment """The signature algorithm is used to specify the cryptographic signature function to use when digitally signing the digest data. Typically, text to be signed goes through three steps: 1) canonicalization, 2) digest, and 3) signature. This property is used to specify the algorithm that should be used for step #3. A signature class typically specifies a default signature algorithm, so this property rarely needs to be used in practice when specifying digital signatures."""@en ;
    rdfs:isDefinedBy cred: ;
.

sec:service a rdf:Property, owl:DeprecatedProperty, owl:ObjectProperty ;
    owl:deprecated true ;
    rdfs:domain sec:Signature ;
    rdfs:range  ;
    rdfs:label "Service" ;
    rdfs:comment """Examples of specific services include discovery services, social networks, file storage services, and verifiable claim repository services."""@en ;
    rdfs:isDefinedBy cred: ;
.

sec:serviceEndpoint a rdf:Property, owl:DeprecatedProperty, owl:ObjectProperty ;
    owl:deprecated true ;
    rdfs:domain sec:Signature ;
    rdfs:range  ;
    rdfs:label "Service endpoint" ;
    rdfs:comment """A network address at which a service operates on behalf of a controller. Examples of specific services include discovery services, social networks, file storage services, and verifiable claim repository services. Service endpoints might also be provided by a generalized data interchange protocol, such as extensible data interchange."""@en ;
    rdfs:isDefinedBy cred: ;
.

sec:x509CertificateChain a rdf:Property, owl:DeprecatedProperty ;
    owl:deprecated true ;
    rdfs:domain sec:Signature ;
    rdfs:range sec:Signature ;
    rdfs:label "X509 Certificate chain" ;
    rdfs:comment """The x509CertificateChain property is used to associate a chain of X.509 Certificates with a proof. The value of this property is an ordered list where each value in the list is an X.509 Certificate expressed as a DER PKIX format, that is encoded with multibase using the base64pad variant. The certificate directly associated to the verification method used to verify the proof MUST be the first element in the list. Subsequent certificates in the list MAY be included where each one MUST certify the previous one."""@en ;
    rdfs:isDefinedBy cred: ;
    rdfs:seeAlso <https://tools.ietf.org/html/rfc5280>, <https://tools.ietf.org/id/draft-multiformats-multibase-00.html> ;
.

sec:x509CertificateFingerprint a rdf:Property, owl:DeprecatedProperty ;
    owl:deprecated true ;
    rdfs:domain sec:Signature ;
    rdfs:range sec:Signature ;
    rdfs:label "X509 Certificate fingerprint" ;
    rdfs:comment """The x509CertificateFingerprint property is used to associate an X.509 Certificate with a proof via its fingerprint. The value is a multihash encoded then multibase encoded value using the base64pad variant. It is RECOMMENDED that the fingerprint value be the SHA-256 hash of the X.509 Certificate."""@en ;
    rdfs:isDefinedBy cred: ;
    rdfs:seeAlso <https://tools.ietf.org/html/rfc5280>, <https://tools.ietf.org/id/draft-multiformats-multibase-00.html> ;
.

sec:allowedAction a rdf:Property, owl:DeprecatedProperty ;
    owl:deprecated true ;
    rdfs:label "Allowed action" ;
    rdfs:comment """An action that the controller of a capability may take when invoking the capability."""@en ;
    rdfs:isDefinedBy cred: ;
    rdfs:seeAlso <https://w3c-ccg.github.io/zcap-spec/#delegated-capability> ;
.

sec:capabilityChain a rdf:Property, owl:DeprecatedProperty ;
    owl:deprecated true ;
    rdfs:label "Capability chain" ;
    rdfs:comment """An list of delegated capabilities from a delegator to a delegatee."""@en ;
    rdfs:isDefinedBy cred: ;
    rdfs:seeAlso <https://w3c-ccg.github.io/zcap-spec/#delegation> ;
.

sec:capabilityAction a rdf:Property, owl:DeprecatedProperty ;
    owl:deprecated true ;
    rdfs:label "Capability action" ;
    rdfs:comment """An action that can be taken given a capability."""@en ;
    rdfs:isDefinedBy cred: ;
    rdfs:seeAlso <https://w3c-ccg.github.io/zcap-spec/#invoking-root-capability> ;
.

sec:caveat a rdf:Property, owl:DeprecatedProperty ;
    owl:deprecated true ;
    rdfs:label "Caveat" ;
    rdfs:comment """A restriction on the way the capability may be used."""@en ;
    rdfs:isDefinedBy cred: ;
    rdfs:seeAlso <https://w3c-ccg.github.io/zcap-spec/#caveats> ;
.

sec:delegator a rdf:Property, owl:DeprecatedProperty ;
    owl:deprecated true ;
    rdfs:label "Delegator" ;
    rdfs:comment """An entity that delegates a capability to a delegatee."""@en ;
    rdfs:isDefinedBy cred: ;
    rdfs:seeAlso <https://w3c-ccg.github.io/zcap-spec/#delegation> ;
.

sec:invocationTarget a rdf:Property, owl:DeprecatedProperty ;
    owl:deprecated true ;
    rdfs:label "Invocation target" ;
    rdfs:comment """An invocation target identifies where a capability may be invoked, and identifies the target object for which the root capability expresses authority."""@en ;
    rdfs:isDefinedBy cred: ;
    rdfs:seeAlso <https://w3c-ccg.github.io/zcap-spec/#root-capability> ;
.

sec:invoker a rdf:Property, owl:DeprecatedProperty ;
    owl:deprecated true ;
    rdfs:label "Invoker" ;
    rdfs:comment """An identifier to cryptographic material that can invoke a capability."""@en ;
    rdfs:isDefinedBy cred: ;
    rdfs:seeAlso <https://w3c-ccg.github.io/zcap-spec/#invocation> ;
.

